Add unused_var_not_matter

ltl.v
@@ -994,3 +994,170 @@ Qed.
 End NormalizeStoreX.
 
 End NormalForms.
+
+(* Unused variables are not matter *)
+
+Section UnusedVar.
+
+Inductive unusedVar (v : Var)
+  : ltl -> Prop :=
+  | unusedVar_VAR (v1 : Var) :
+      v <> v1 -> unusedVar v (var v1)
+  | unusedVar_OR (p1 p2 : ltl) :
+      unusedVar v p1 ->
+      unusedVar v p2 ->
+      unusedVar v (p1 .\/ p2)
+  | unusedVar_STORE_X (R : list register) (psi : ltl) (phi : ltl_phi) :
+      unusedVar v psi ->
+      unusedVar v (↓ R,X psi ../\ phi)
+  | unusedVar_PHI (phi : ltl_phi) :
+      unusedVar v (φ phi)
+  .
+
+Variables sigma1 sigma2 : eqn_sys.
+Variable vs : list Var.
+Hypothesis vs_not_in_sigma1 :
+  forall v, List.In v vs -> forall v', unusedVar v (sigma1 v').
+Hypothesis sigma_equiv :
+  forall v, ~ List.In v vs -> sigma1 v = sigma2 v.
+
+Lemma unused_var_not_matter :
+  forall ell i j theta theta' x,
+  forall v, ~ List.In v vs ->
+    Fpow_emp sigma1 ell v i j theta theta' x
+    <-> Fpow_emp sigma2 ell v i j theta theta' x.
+Proof.
+  intros ell.
+  induction ell as [| ell IH];
+    intros i j theta theta' x v Hv.
+  - (* base case (ell = 0) *)
+    unfold Fpow_emp, Fpow.
+    reflexivity.
+  - (* inductive step on ell *)
+    assert (vs_not_in_sigma1_v:
+      forall v1, List.In v1 vs ->
+        unusedVar v1 (sigma1 v)).
+    {
+      intros v1 Hv1.
+      now apply vs_not_in_sigma1.
+    }
+    clear vs_not_in_sigma1.
+    unfold Fpow_emp, Fpow, F.
+    rewrite <- (sigma_equiv v Hv).
+
+    split;
+    intros H;
+    destruct H as [H | H];
+    [ left | (right; apply H)
+    | left | (right; apply H)];
+    generalize dependent x;
+    generalize dependent theta';
+    generalize dependent theta;
+    generalize dependent j;
+    generalize dependent i;
+
+    induction (sigma1 v) as [v'
+      | l1 IH1 l2 IH2 | R l1 IH1 phi | phi];
+      intros i j th th' x H.
+    + (* when sigma1 v = var v' *)
+      assert (Hnv': ~ List.In v' vs).
+      {
+        intros Hv'.
+        specialize (vs_not_in_sigma1_v v' Hv').
+        inversion vs_not_in_sigma1_v as [v'' nEQv' | | |].
+        now apply nEQv'.
+      }
+      inversion H;
+      apply models_fin_var; auto;
+      apply IH; auto.
+    + (* when sigma1 v = l1 .\/ l2 *)
+      assert (Hnvl1 : forall v1, List.In v1 vs -> unusedVar v1 l1).
+      {
+        intros v1 Hv1.
+        specialize (vs_not_in_sigma1_v v1 Hv1).
+        now inversion vs_not_in_sigma1_v.
+      }
+      assert (Hnvl2 : forall v1, List.In v1 vs -> unusedVar v1 l2).
+      {
+        intros v1 Hv1.
+        specialize (vs_not_in_sigma1_v v1 Hv1).
+        now inversion vs_not_in_sigma1_v.
+      }
+      inversion_clear H as [
+        | i' j' th1 th2 x' l1' l2' Hij H' EQi' EQj' EQth1 EQth2 EQx' [EQl1' EQl2']
+        | | |];
+      apply models_fin_OR; auto.
+      destruct H' as [H | H];
+      [left | right];
+      [apply IH1 | apply IH2]; auto.
+    + (* when sigma1 v = ↓ R,X l1 ../\ phi *)
+      assert (Hnvl1 : forall v1, List.In v1 vs -> unusedVar v1 l1).
+      {
+        intros v1 Hv1.
+        specialize (vs_not_in_sigma1_v v1 Hv1).
+        now inversion vs_not_in_sigma1_v.
+      }
+      inversion_clear H as [|
+        | i' j' th1 th2 x' R' l1' phi' Hij Hphi H'
+          EQi' EQj' EQth1 EQth2 EQx' [EQR' EQl1' EQphi'] | |];
+      apply models_fin_STORE_X; auto.
+    + (* when sigma1 v = φ phi *)
+      inversion_clear H as [| |
+       | i' j' th1 Hij | i' j' th1 phi' nphitt Hij Hphi].
+      * (* when phi = [tt] *)
+        apply models_fin_TT; auto.
+      * (* when phi <> [tt] *)
+        apply models_fin_PHI; auto.
+
+    + (* when sigma1 v = var v', for <- *)
+      assert (Hnv': ~ List.In v' vs).
+      {
+        intros Hv'.
+        specialize (vs_not_in_sigma1_v v' Hv').
+        inversion vs_not_in_sigma1_v as [v'' nEQv' | | |].
+        now apply nEQv'.
+      }
+      inversion H;
+      apply models_fin_var; auto;
+      apply IH; auto.
+    + (* when sigma1 v = l1 .\/ l2, for <- *)
+      assert (Hnvl1 : forall v1, List.In v1 vs -> unusedVar v1 l1).
+      {
+        intros v1 Hv1.
+        specialize (vs_not_in_sigma1_v v1 Hv1).
+        now inversion vs_not_in_sigma1_v.
+      }
+      assert (Hnvl2 : forall v1, List.In v1 vs -> unusedVar v1 l2).
+      {
+        intros v1 Hv1.
+        specialize (vs_not_in_sigma1_v v1 Hv1).
+        now inversion vs_not_in_sigma1_v.
+      }
+      inversion_clear H as [
+        | i' j' th1 th2 x' l1' l2' Hij H' EQi' EQj' EQth1 EQth2 EQx' [EQl1' EQl2']
+        | | |];
+      apply models_fin_OR; auto.
+      destruct H' as [H | H];
+      [left | right];
+      [apply IH1 | apply IH2]; auto.
+    + (* when sigma1 v = ↓ R,X l1 ../\ phi, for <- *)
+      assert (Hnvl1 : forall v1, List.In v1 vs -> unusedVar v1 l1).
+      {
+        intros v1 Hv1.
+        specialize (vs_not_in_sigma1_v v1 Hv1).
+        now inversion vs_not_in_sigma1_v.
+      }
+      inversion_clear H as [|
+        | i' j' th1 th2 x' R' l1' phi' Hij Hphi H'
+          EQi' EQj' EQth1 EQth2 EQx' [EQR' EQl1' EQphi'] | |];
+      apply models_fin_STORE_X; auto.
+    + (* when sigma1 v = φ phi, for <- *)
+      inversion_clear H as [| |
+       | i' j' th1 Hij | i' j' th1 phi' nphitt Hij Hphi].
+      * (* when phi = [tt] *)
+        apply models_fin_TT; auto.
+      * (* when phi <> [tt] *)
+        apply models_fin_PHI; auto.
+Qed.
+
+End UnusedVar.
